Nearly done. :)

OneTimePad.thy
@@ -3,9 +3,9 @@ theory OneTimePad imports
   "HOL/Groups_Big"
 begin
 
-type_synonym key     = "int list"
-type_synonym message = "int list"
-type_synonym crypted = "int list"
+type_synonym key     = "bool list"
+type_synonym message = "bool list"
+type_synonym crypted = "bool list"
 
 definition zipWith :: "('a \<Rightarrow> 'b \<Rightarrow> 'c) \<Rightarrow> 'a list \<Rightarrow> 'b list \<Rightarrow> 'c list" where
   "zipWith f xs ys = map (\<lambda> (x, y). f x y) (zip xs ys)"
@@ -17,46 +17,48 @@ definition zipWith :: "('a \<Rightarrow> 'b \<Rightarrow> 'c) \<Rightarrow> 'a l
 lemma "length xs = length ys \<Longrightarrow> zipWith f xs ys = map (\<lambda> (x, y). f x y) (zip xs ys)"
 by (induct xs ys rule: list_induct2, auto)*)
 
+definition xor :: "bool \<Rightarrow> bool \<Rightarrow> bool" where
+  "xor = not_equal"
+
 definition encrypt :: "message \<Rightarrow> key \<Rightarrow> crypted" where
-  "encrypt = zipWith plus"
+  "encrypt = zipWith xor"
 
 definition decrypt :: "crypted \<Rightarrow> key \<Rightarrow> message" where
-  "decrypt = zipWith minus"
+  "decrypt = zipWith xor"
   
 definition reconstruct_key :: "crypted \<Rightarrow> message \<Rightarrow> key" where
-  "reconstruct_key = zipWith minus"
+  "reconstruct_key = zipWith xor"
   
 
-lemma "length m = length k \<Longrightarrow> decrypt (encrypt m k) k = m"
-unfolding encrypt_def decrypt_def zipWith_def
-by (induct m k rule: list_induct2, auto)
+lemma enc:
+  assumes "length m = length k"
+    shows "length (encrypt m k) = length m"
+      and "decrypt (encrypt m k) k = m"
+unfolding encrypt_def decrypt_def zipWith_def xor_def
+using assms by (induct m k rule: list_induct2, auto)
 
-lemma "length m = length k \<Longrightarrow> length (encrypt m k) = length m"
-unfolding encrypt_def zipWith_def
-by (induct m k rule: list_induct2, auto)
 
 lemma reconstruct:
   assumes "length m = length c"
     shows "length (reconstruct_key c m) = length m"
       and "encrypt m (reconstruct_key c m) = c"
-unfolding encrypt_def reconstruct_key_def zipWith_def
+unfolding encrypt_def reconstruct_key_def zipWith_def xor_def
 using assms by (induct m c rule: list_induct2, auto)
 
-lemma test:
-  assumes "length m = length c"
-    shows "\<exists>!k. length m = length k \<and> encrypt m k = c"
-proof (intro ex1I)
-  show "length m = length (reconstruct_key c m) \<and>
-        encrypt m (reconstruct_key c m) = c"
-        using reconstruct[OF assms] by auto
-next
-  show "\<And>k. length m = length k \<and> encrypt m k = c \<Longrightarrow> k = reconstruct_key c m"
-  (*unfolding encrypt_def reconstruct_key_def zipWith_def
-  apply (induct m k rule: list_induct2)*)
-  sorry
+lemma rec_uniq:
+  assumes "length m = length k"
+      and "encrypt m k = c"
+    shows "k = reconstruct_key c m"
+proof -
+  have L: "length k = length c" using enc(1) assms(1) assms(2) by auto
+  show ?thesis using assms(1) L assms(2) unfolding encrypt_def reconstruct_key_def zipWith_def xor_def
+    by (induct m k c rule: list_induct3, auto)
 qed
 
-
+lemma uniq_key:
+  assumes "length m = length c"
+    shows "\<exists>!k. length m = length k \<and> encrypt m k = c"
+using reconstruct[OF assms] rec_uniq by (intro ex1I[of _ "reconstruct_key c m"], auto)
 
 axiomatization
       \<K> :: "key set"
@@ -64,38 +66,117 @@ axiomatization
   and P\<^sub>\<K> :: "key pmf"
   and P\<^sub>\<M> :: "message pmf"
   and len :: nat
-where k_finite: "finite \<K>"
-  and m_finite: "finite \<M>"
-  and k_nonemp: "\<K> \<noteq> {}"
-  and m_nonemp: "\<M> \<noteq> {}"
-  and k_length: "\<forall>k\<in>\<K>. length k = len"
-  and m_length: "\<forall>m\<in>\<M>. length m = len"
-  and k_unipmf: "P\<^sub>\<K> = pmf_of_set \<K>"  (* uniform distribution *)
+where k_unipmf: "P\<^sub>\<K> = pmf_of_set \<K>"  (* uniform distribution *)
+  and m_pmf: "set_pmf P\<^sub>\<M> \<subseteq> \<M>"
+  and k_set: "\<K> = set (List.n_lists len [True, False])"
+  and m_set: "\<M> = \<K>"
 
 definition \<P>\<^sub>\<K> :: "key \<Rightarrow> real" where "\<P>\<^sub>\<K> = pmf P\<^sub>\<K>"
 definition \<P>\<^sub>\<M> :: "message \<Rightarrow> real" where "\<P>\<^sub>\<M> = pmf P\<^sub>\<M>"
 
-lemma "k \<in> \<K> \<Longrightarrow> \<P>\<^sub>\<K> k = 1 / card \<K>"
+lemma k_finite: "finite \<K>"
+by (metis List.finite_set k_set)
+
+lemma k_nonemp: "\<K> \<noteq> {}"
+unfolding k_set set_n_lists by (simp add: Ex_list_of_length subsetI)
+
+lemma k_length: "\<forall>k\<in>\<K>. length k = len"
+unfolding k_set using length_n_lists_elem by auto
+
+lemma k_in_k: "k \<in> \<K> \<longleftrightarrow> (length k = len)"
+proof (rule iffI)
+  assume "k \<in> \<K>"
+  then show "length k = len" unfolding k_set using length_n_lists_elem by auto
+next
+  assume "length k = len"
+  then show "k \<in> \<K>" unfolding k_set set_n_lists by auto
+qed
+
+lemma pmf_sum_one:
+  assumes "finite M"
+      and "set_pmf P \<subseteq> M"
+    shows "(\<Sum>m\<in>M. pmf P m) = 1"
+proof -
+  have "(\<Sum>m\<in>M. pmf P m) = measure (measure_pmf P) M"
+    using assms(1) by (simp add: measure_measure_pmf_finite)
+  show ?thesis sorry
+qed
+
+lemma m_sum_one: "(\<Sum>m\<in>\<M>. \<P>\<^sub>\<M> m) = 1"
+using pmf_sum_one[of \<M> P\<^sub>\<M>] k_finite m_pmf unfolding \<P>\<^sub>\<M>_def m_set by auto
+
+
+lemma k_prob: "k \<in> \<K> \<Longrightarrow> \<P>\<^sub>\<K> k = 1 / card \<K>"
 unfolding \<P>\<^sub>\<K>_def k_unipmf pmf_of_set[OF k_nonemp k_finite] by auto
 
 
 (* probability of cryptogram c if message m is chosen *)
 definition \<P>\<^sub>\<M>\<^sub>\<C> :: "message \<Rightarrow> crypted \<Rightarrow> real" where
-  "\<P>\<^sub>\<M>\<^sub>\<C> m c = (\<Sum>k | k\<in>\<K> \<and> length k = length m \<and> encrypt m k = c. \<P>\<^sub>\<K> k)"
+  "\<P>\<^sub>\<M>\<^sub>\<C> m c = (\<Sum>k | k \<in> \<K> \<and> encrypt m k = c. \<P>\<^sub>\<K> k)"
 
-lemma "\<P>\<^sub>\<M>\<^sub>\<C> m c = 1 / card \<K>"
-sorry
+lemma set_singleton:
+  assumes "\<forall>x \<in> S. (P x \<longrightarrow> x = y)"
+      and "\<exists>x \<in> S.  P x"
+    shows "{x \<in> S. P x} = {y}"
+by (smt Collect_cong Set.ball_empty assms insert_compr)
+
+lemma rec_in_k:
+  assumes "m \<in> \<M>"
+      and "length m = length c"
+    shows "reconstruct_key c m \<in> \<K>"
+proof -
+  have "length m = len" using assms(1) k_length m_set by auto
+  then have "length (reconstruct_key c m) = len" using reconstruct(1)[OF assms(2)] by auto
+  then show ?thesis using k_in_k by auto
+qed
+
+lemma uniq_k:
+  assumes "m \<in> \<M>"
+      and "length m = length c"
+    shows "{k \<in> \<K>. encrypt m k = c} = {reconstruct_key c m}"
+proof (rule set_singleton)
+  show "\<exists>k\<in>\<K>. encrypt m k = c"
+  proof (rule bexI[of _ "reconstruct_key c m"])
+    show "encrypt m (reconstruct_key c m) = c" using reconstruct(2)[OF assms(2)] .
+    show "reconstruct_key c m \<in> \<K>" using rec_in_k[OF assms] by auto
+  qed
+  show "\<forall>k\<in>\<K>. encrypt m k = c \<longrightarrow> k = reconstruct_key c m"
+  proof (rule ballI)
+    fix k
+    assume K: "k \<in> \<K>"
+    then have "length k = len" using k_in_k by auto
+    also have "length m = len" using assms(1) k_in_k unfolding m_set by auto
+    finally have "length m = length k" .
+    then show "encrypt m k = c \<longrightarrow> k = reconstruct_key c m" using rec_uniq by auto
+  qed
+qed
+
+lemma pmc_card_k:
+  assumes "m \<in> \<M>"
+      and "length c = len"
+    shows "\<P>\<^sub>\<M>\<^sub>\<C> m c = 1 / card \<K>"
+proof -
+  have L: "length m = length c" using k_in_k m_set assms by auto
+  have K: "(reconstruct_key c m) \<in> \<K>" using rec_in_k[OF assms(1) L] .
+  have "\<P>\<^sub>\<K> (reconstruct_key c m) = 1 / real (card \<K>)" using k_prob[OF K] .
+  then show ?thesis unfolding \<P>\<^sub>\<M>\<^sub>\<C>_def unfolding uniq_k[OF assms(1) L] by simp
+qed
 
 (* probability of obtaining cryptogram c from any cause *)
 definition \<P>\<^sub>\<C> :: "crypted \<Rightarrow> real" where
   "\<P>\<^sub>\<C> c = (\<Sum>m\<in>\<M>. \<P>\<^sub>\<M> m * \<P>\<^sub>\<M>\<^sub>\<C> m c)"
 
-theorem "\<P>\<^sub>\<M>\<^sub>\<C> m c = \<P>\<^sub>\<C> c"
-sorry
-
-
-(*theorem "\<lbrakk> length m = length k; length m = length k'; m \<noteq> []; c = encrypt m k; k \<noteq> k' \<rbrakk>
-  \<Longrightarrow> decrypt c k' \<noteq> m"*)
-
+theorem
+  assumes "m \<in> \<M>"
+      and "length c = len"
+    shows "\<P>\<^sub>\<M>\<^sub>\<C> m c = \<P>\<^sub>\<C> c"
+proof -
+  have "\<P>\<^sub>\<C> c = (\<Sum>m\<in>\<M>. \<P>\<^sub>\<M> m * \<P>\<^sub>\<M>\<^sub>\<C> m c)" unfolding \<P>\<^sub>\<C>_def by auto
+  also have "... = (\<Sum>m\<in>\<M>. \<P>\<^sub>\<M> m * 1 / card \<K>)" using pmc_card_k[OF _ assms(2)] by auto
+  also have "... = (\<Sum>m\<in>\<M>. \<P>\<^sub>\<M> m) / card \<K>" by (smt setsum.cong setsum_divide_distrib)
+  also have "... = 1 / card \<K>" using m_sum_one by simp
+  finally have "\<P>\<^sub>\<C> c = 1 / real (card \<K>)" by auto
+  then show ?thesis using pmc_card_k[OF assms] by simp
+qed
 
 end
